Word.v
@@ -1,0 +1,23 @@
+Section WORD.
+
+  Variable A : Type.
+
+  Inductive Alphabet : Type :=
+  | Pe: A -> Alphabet
+  | Ne: A -> Alphabet.
+
+  Definition Word := list Alphabet.
+
+  Definition opposite (letter: Alphabet) : Alphabet :=
+    match letter with
+    | Pe x => Ne x
+    | Ne x => Pe x
+    end.
+
+  Lemma double_opposite: forall a, opposite (opposite a) = a.
+  Proof. intros. destruct a; simpl; auto. Qed.
+
+End WORD.
+
+Arguments Pe [_] _.
+Arguments Ne [_] _.
